\documentclass[12pt]{article}
\usepackage{fullpage,url,amssymb,epsfig,color,xspace,tikz,amsmath}

\begin{document}

\begin{align*}
    E(\tilde{\theta}) & = E(\tilde{\tau_{2}} + \bar{Y}) \\
    & = E(\tilde{\tau_{2}}) + E(\bar{Y}) \\
    & = \tau_2 + \mu \text{\quad since unbiased}
\end{align*}

\begin{align*}
    Var(\tilde{\theta}) & = Var(\tilde{\tau_{2}} + \bar{Y}) \\
    & = Var(\bar{Y_2} - \bar{Y} + \bar{Y}) \\
    & = Var(\bar{Y_2}) \\
    & = \frac {\sigma^2} {4} 
\end{align*}
So,
\begin{align*}
    d & = \frac {\hat{\theta} - 30} {se(\tilde{\theta})} \\
    & = \frac {25.25 - 30} {2.939 / \sqrt{4}} \\
    & = -3.232392
\end{align*}

\begin{align*}
    E(\tilde{\theta}) & = E(\tilde{\tau_1}) - 2 E(\tilde{\tau_2}) + E(\tilde{\tau_3}) \\
    & = \tau_1 - 2 \tau_2 + \tau_3 \text{\quad since unbiased}
\end{align*}
and, 
\begin{align*}
    Var(\tilde{\theta}) & = Var(\tilde{\tau_1} - 2 \tilde{\tau_2} + \tilde{\tau_3}) \\
    & = Var(\tilde{\tau_1}) + 4 Var(\tilde{\tau_2}) + Var(\tilde{\tau_3}) \\
    & = \frac {\sigma^2} {4} + \sigma^2 + \frac {\sigma^2} {4} \\
    & = \frac 3 2 \sigma^2
\end{align*}
So,
\begin{align*}
    d & = \frac {\hat{\tau_1} - 2 \hat{\tau_2} + \hat{\tau_3} - 0} {\frac 3 2 \hat{\sigma}^2}\\
    & = 2 \frac {4.25 - 2 \times 6.5 - (4.25 + 6.5)} {3 \times 2.939} \\
    & = -4.423273
\end{align*}
\end{document}