\documentclass[12pt]{article}
\usepackage{amsmath}
\begin{document}
Let $X_{aug} = \sqrt{\lambda} I_{p \times p}$ and $Y_{aug} = \vec{0}_{p \times p}$.\\
So 
\begin{align*}
    X^* &= 
    \begin{bmatrix}
        x_{1} \\
       x_{2} \\
       \vdots \\
       X_{aug}
    \end{bmatrix}
\end{align*}
where $x_i = [x_{i1}, \cdots, x_{ip}]$\\
and 
\begin{align*}
    Y^* &= 
    \begin{bmatrix}
        Y_{1} \\
       Y_{2} \\
       \vdots \\
       Y_{aug}
    \end{bmatrix}
\end{align*}
Let $n' = n + dim(X_{aug})$\\
Hence, 
\begin{align*}
    Rss(\lambda) & = \sum_{i = 1}^{n'}(Y^*_i - X^* \beta)^2\\
    & = \sum_{i = 1}^{n'}(Y_i - \beta_1 x_{i1} - \cdots - \beta_n x_{ip})^2\\
    & = \sum_{i = 1}^{n}(Y_i - X \beta)^2 + (0 - \sqrt{\lambda} \beta_1)^2 + \cdots + (0 - \sqrt{\lambda} \beta_p)^2\\
    & = \sum_{i = 1}^{n}(Y_i - X \beta)^2 + \lambda \sum_{j = 1}^p \beta_j^2
\end{align*}
Since, $Rss(\lambda) = Rss_{Ridge}(\lambda)$, \\
$\hat \beta_{Ridge} = ({X^*}^T X^*)^{-1} {X^*}^T Y^* = ({X}^T X + \lambda I)^{-1} {X}^T Y$
\end{document}