\documentclass[12pt]{article}
\usepackage{fullpage,url,amssymb,epsfig,color,xspace,tikz,amsmath, amsthm}
\begin{document}

\begin{proof}
    We first prove $\frac{1}{N_\mathcal{S}} \sum_{j=1}^{N_\mathcal{S}} \frac{1}{N} \sum_{i \in \mathcal{P}} (\widehat{\mu}_{\mathcal{S}_j}({\mathbf{x}_i}) - \overline{\widehat{\mu}}({\mathbf{x}_i}))
(\overline{\widehat{\mu}}({\mathbf{x}_i}) - {\mu}({\mathbf{x}_i})) = 0$.\\
Let $P = \cup_{i = 1}^{k} A_i$ where $A_i=\{u : u \in P, x_u=x_i\}$ and the unique value of $\mathbf{x}$ is $\mathbf{x}_1, \dots, \mathbf{x}_k$.\\
$\lvert A_i \rvert = n_i$ for all $1 \leq i \leq k$
\begin{align*}
    &\frac{1}{N_\mathcal{S}} \sum_{j=1}^{N_\mathcal{S}} \frac{1}{N} \sum_{i \in \mathcal{P}} (\widehat{\mu}_{\mathcal{S}_j}({\mathbf{x}_i}) - \overline{\widehat{\mu}}({\mathbf{x}_i}))
    (\overline{\widehat{\mu}}({\mathbf{x}_i}) - {\mu}({\mathbf{x}_i}))\\
    = & \frac {1} {N_\mathcal{S} N} \sum_{j=1}^{N_\mathcal{S}} [\sum_{i \in A_1} (\widehat{\mu}_{\mathcal{S}_j}({\mathbf{x}_i}) - \overline{\widehat{\mu}}({\mathbf{x}_i}))
    (\overline{\widehat{\mu}}({\mathbf{x}_i}) - {\mu}({\mathbf{x}_i})) + \dots + \sum_{i \in A_k}(\widehat{\mu}_{\mathcal{S}_j}({\mathbf{x}_i}) - \overline{\widehat{\mu}}({\mathbf{x}_i}))
    (\overline{\widehat{\mu}}({\mathbf{x}_i}) - {\mu}({\mathbf{x}_i}))]
\end{align*}
For $i \in A_m$ where $1 \leq m \leq k$, we have,
\begin{align*}
    & \frac {1} {N_\mathcal{S} N} \sum_{j=1}^{N_\mathcal{S}} \sum_{i \in A_m} (\widehat{\mu}_{\mathcal{S}_j}({\mathbf{x}_i}) - 
    \overline{\widehat{\mu}}({\mathbf{x}_i})) (\overline{\widehat{\mu}}({\mathbf{x}_i}) - {\mu}({\mathbf{x}_i}))\\
    = & \frac {1} {N_\mathcal{S} N} \sum_{j=1}^{N_\mathcal{S}} \sum_{i \in A_m} \widehat{\mu}_{\mathcal{S}_j}({\mathbf{x}_i}) \overline{\widehat{\mu}}({\mathbf{x}_i})
        - \frac {1} {N_\mathcal{S} N} \sum_{j=1}^{N_\mathcal{S}} \sum_{i \in A_m} \widehat{\mu}_{\mathcal{S}_j}({\mathbf{x}_i}) {\mu}({\mathbf{x}_i})\\
       & - \frac {1} {N_\mathcal{S} N} \sum_{j=1}^{N_\mathcal{S}} \sum_{i \in A_m} \overline{\widehat{\mu}}({\mathbf{x}_i})^2
        +  \frac {1} {N_\mathcal{S} N} \sum_{j=1}^{N_\mathcal{S}} \overline{\widehat{\mu}}({\mathbf{x}_i}) {\mu}({\mathbf{x}_i})\\
    = & \frac {1} {N} \sum_{i \in A_m} \frac {\overline{\widehat{\mu}}(\mathbf{x}_i)} {N_\mathcal{S}} \sum_{j=1}^{N_\mathcal{S}} \widehat{\mu}_{\mathcal{S}_j}({\mathbf{x}_i})
        - \frac {1} {N} \sum_{i \in A_m} \frac {{\mu}(\mathbf{x}_i)} {N_\mathcal{S}} \sum_{j=1}^{N_\mathcal{S}} \widehat{\mu}_{\mathcal{S}_j}({\mathbf{x}_i})
        - \frac {1} {N} \sum_{i \in A_m} \overline{\widehat{\mu}}({\mathbf{x}_i})^2 + \frac {1} {N} \sum_{i \in A_m} \overline{\widehat{\mu}}({\mathbf{x}_i}) {\mu}({\mathbf{x}_i})\\
    = & \frac {1} {N} \sum_{i \in A_m} \overline{\widehat{\mu}}({\mathbf{x}_i})^2 - \frac {1} {N} \sum_{i \in A_m} \overline{\widehat{\mu}}({\mathbf{x}_i})^2 +
    \frac {1} {N} \sum_{i \in A_m} \overline{\widehat{\mu}}({\mathbf{x}_i}) {\mu}({\mathbf{x}_i}) - \frac {1} {N} \sum_{i \in A_m} \overline{\widehat{\mu}}({\mathbf{x}_i}) {\mu}({\mathbf{x}_i})\\
    = & 0
\end{align*}
So, $\frac{1}{N_\mathcal{S}} \sum_{j=1}^{N_\mathcal{S}} \frac{1}{N} \sum_{i \in \mathcal{P}} (\widehat{\mu}_{\mathcal{S}_j}({\mathbf{x}_i}) - \overline{\widehat{\mu}}({\mathbf{x}_i}))
(\overline{\widehat{\mu}}({\mathbf{x}_i}) - {\mu}({\mathbf{x}_i})) = 0$\\
Hence, we have,
\begin{align*}
    & \frac{1}{N_\mathcal{S}} \sum_{j=1}^{N_\mathcal{S}} \frac{1}{N}\sum_{i \in \mathcal{P}} (\widehat{\mu}_{\mathcal{S}_j}({\mathbf{x}_i}) - {\mu}({\mathbf{x}_i}))^2\\
    = & \frac{1}{N_\mathcal{S}} \sum_{j=1}^{N_\mathcal{S}} \frac{1}{N}\sum_{i \in \mathcal{P}} 
    (\widehat{\mu}_{\mathcal{S}_j}({\mathbf{x}_i}) - \overline{\widehat{\mu}}({\mathbf{x}_i}) + \overline{\widehat{\mu}}({\mathbf{x}_i}) - {\mu}({\mathbf{x}_i}))^2\\
    = & \frac{1}{N_\mathcal{S}} \sum_{j=1}^{N_\mathcal{S}} \frac{1}{N}\sum_{i \in \mathcal{P}} 
    (\widehat{\mu}_{\mathcal{S}_j}({\mathbf{x}_i}) - \overline{\widehat{\mu}}({\mathbf{x}_i}))^2 + (\overline{\widehat{\mu}}({\mathbf{x}_i}) - {\mu}({\mathbf{x}_i}))^2
    + 2(\widehat{\mu}_{\mathcal{S}_j}({\mathbf{x}_i}) - \overline{\widehat{\mu}}({\mathbf{x}_i}))
    (\overline{\widehat{\mu}}({\mathbf{x}_i}) - {\mu}({\mathbf{x}_i}))\\
    = & \frac{1}{N_\mathcal{S}} \sum_{j=1}^{N_\mathcal{S}} \frac{1}{N}\sum_{i \in \mathcal{P}} (\widehat{\mu}_{\mathcal{S}_j}({\mathbf{x}_i}) - \overline{\widehat{\mu}}({\mathbf{x}_i}))^2 + 
    \frac{1}{N_\mathcal{S}} \sum_{j=1}^{N_\mathcal{S}} \frac{1}{N}\sum_{i \in \mathcal{P}} (\overline{\widehat{\mu}}({\mathbf{x}_i}) - {\mu}({\mathbf{x}_i}))^2\\
\end{align*}
\end{proof}



\end{document}