---
title: "a1q1"
author: "Mushi Wang"
date: "02/06/2020"
output: pdf_document
---

**q1**
(a)
Let $\beta = (\beta_1, \beta_2, \dots, \beta_n)^T$, $X = (x_1, x_2, \dots, x_n)^T$ and $\Sigma$ be variance-covariance matrix.
\begin{align*}
E(\tilde{\beta}_{WLS}) &= E((X^T W X)^{-1}X^T WY)\\
  & = (X^T W X)^{-1}X^T W E(Y)\\
  & = (X^T W X)^{-1}X^T W E(X\beta + \epsilon)\\
  & = (X^T W X)^{-1}X^T W XE(\beta) + (X^T W X)^{-1}XW E(\epsilon)\\
  & = (X^T W X)^{-1}X^T W X \beta + 0 \quad\quad (E(\epsilon) = 0)\\
  & = \beta
\end{align*}

\newpage
(b)
Let $W = diag(\frac {1} {g(x_1)}, \frac {1} {g(x_n)}, \dots, \frac {1} {g(x_n)})$.
So $W^T = W$.\
Since $\Sigma = \sigma^2 diag(g(x_1), g(x_2), \dots, g(x_n))$, so $\Sigma \times W = \sigma^2$
\begin{align*}
  Var(\tilde{\beta}_{WLS}) & = Var((X^T W X)^{-1}XWY)\\
  & = (X^T W X)^{-1}X^T W \times Var(Y) \times ((X^T W X)^{-1}X^T W)^T\\
  & = (X^T W X)^{-1}X^T W \times Var(X\beta + \epsilon) \times ((X^T W X)^{-1}X^T W)^T\\
  & = (X^T W X)^{-1}X^T W \times Var(\epsilon) \times W^T X (X^T W^T X)^{-1}\\
  & = (X^T W X)^{-1}X^T W \times \Sigma \times W^T X (X^T W^T X)^{-1}\\
  & = \sigma^2 (X^T W X)^{-1}X^T W X (X^T W^T X)^{-1}\\
  & = \sigma^2 (X^T W X)^{-1}
\end{align*}